...

theories/types.v
@@ -39,32 +39,7 @@ Definition insert' {A} b (y: A) (m: gmap string A) :=
   match b with BNamed x => <[x:=y]>m | BAnon => m end.
 Definition Let b e e' := App (Rec BAnon b e') e.
 
-(* TODO - figure out how to get a nice notation working. *)
-Inductive typing: lnames → env → expr → hexpr → lnames → type → hexpr → Prop :=
-| tytrue U Γ: typing U Γ Ctrue ∅ ∅ Bool ∅
-| tyfalse U Γ: typing U Γ Cfalse ∅ ∅ Bool ∅
-| tyunit  U Γ: typing U Γ Cunit ∅ ∅ Unit ∅
-| tyvar U Γ (x: string) τ (Γx: Γ !! x = Some τ): typing U Γ x ∅ ∅ τ ∅
-| tylet U Γ (x: binder) η₁ η₂ η₃ τ₁ τ₂ A₁ A₂ e₁ e₂:
-    typing U Γ e₁ η₁ A₁ τ₁ η₂ →
-    typing (U ∪ A₁) (insert' x τ₁ Γ) e₂ η₂ A₂ τ₂ η₃ →
-    typing U Γ (Let x e₁ e₂) η₁ (A₁ ∪ A₂) τ₂ η₃
-| tyref U Γ e η₁ η₂ τ A ξ (ξ_fresh: ξ ∉ U ∪ A):
-    typing U Γ e η₁ A τ η₂ →
-    typing U Γ (Alloc e) η₁ (A ∪ {[ ξ ]}) (Ref(ξ)) (η₂ ⊗ ξ ↦ τ)
-| tyread U Γ e η₁ η₂ ξ τ A:
-    typing U Γ e η₁ A (Ref(ξ)) (η₂ ⊗ ξ ↦ τ) →
-    typing U Γ (Read e) η₁ A τ (η₂ ⊗ ξ ↦ τ)
-| tywrite U Γ e e' η₁ η₂ η₃ ξ τ A₁ A₂:
-    typing U Γ e η₁ A₁ (Ref(ξ)) η₂ →
-    typing (U ∪ A₁) Γ e' η₂ A₂ τ (η₃ ⊗ ξ ↦ τ) →
-    typing U Γ (Write e e') η₁ (A₁ ∪ A₂) Unit (η₃ ⊗ ξ ↦ τ)
-| typost U Γ e η₁ η₂ τ A ξ (ξ_fresh: ξ ∉ U ∪ A):
-    typing U Γ e η₁ A τ η₂ →
-    typing U Γ (Post e) η₁ {[ξ]} (Promise(ξ,A) τ) (Wait(ξ,A) η₂).
-
 Class Names A := names: A → gset lname.
-
 Fixpoint ty_names τ: gset lname :=
   match τ with
   | tbool => ∅
@@ -78,10 +53,68 @@ Fixpoint he_names η: gset lname :=
   match η with
   | hemp => ∅
   | hstar η η' => he_names η ∪ he_names η'
-  | hpt ξ τ => {[ ξ ]} ∪ ty_names τ
+  | hpt ξ τ => {[ ξ ]} ∪ names τ
   | hwait ξ A η => {[ ξ ]} ∪ (he_names η ∖ A)
   end.
 Instance: Names hexpr := he_names.
+
+Fixpoint res_names η: gset lname :=
+  match η with
+  | hemp => ∅
+  | hstar η η' => res_names η ∪ res_names η'
+  | hpt ξ τ => {[ ξ ]}
+  | hwait ξ A η => {[ ξ ]} ∪ (res_names η ∖ A)
+  end.
+         
+Inductive hexpr_equiv: Equiv hexpr :=
+| hee_refl: Reflexive (≡)
+| hee_symm: Symmetric (≡)
+| hee_trans: Transitive (≡)
+| hee_proper_star: Proper ((≡) ==> (≡) ==> (≡)) hstar
+| hee_proper_wait: ∀ ξ A, Proper ((≡) ==> (≡)) (hwait ξ A)
+| hee_assoc: Assoc (≡) hstar
+| hee_comm: Comm (≡) hstar
+| hee_left: LeftId (≡) hemp hstar.
+Instance hexpr_equivalence: Equivalence hexpr_equiv.
+Proof. split; [apply hee_refl|apply hee_symm|apply hee_trans]. Qed.
+Existing Instances hee_proper_star hee_proper_wait hee_assoc hee_comm hee_left hexpr_equiv.
+Instance: RightId (≡) hemp hstar.
+Proof. intro; rewrite comm left_id //. Qed.
+
+Instance he_names_proper: Proper ((≡) ==> (=)) he_names.
+Proof.
+  intros η η' eqη.
+  apply leibniz_equiv.
+  induction eqη; simpl; try done.
+  - by etrans.
+  - by f_equiv.
+  - by do 2 f_equiv.
+  - by rewrite assoc.
+  - by rewrite comm.
+  - by rewrite left_id.
+Qed.
+
+Instance res_names_proper: Proper ((≡) ==> (=)) res_names.
+Proof.
+  intros η η' eqη.
+  apply leibniz_equiv.
+  induction eqη; simpl; try done.
+  - by etrans.
+  - by f_equiv.
+  - by do 2 f_equiv.
+  - by rewrite assoc.
+  - by rewrite comm.
+  - by rewrite left_id.
+Qed.
+
+Lemma res_names_sub_names η: res_names η ⊆ names η.
+Proof.
+  induction η; cbn -[union]; try done.
+  - by apply union_mono.
+  - apply union_subseteq_l.
+  - apply union_mono; first done.
+    apply difference_mono; done.
+Qed.
 
 Instance combine_names `{Names A, Names B}: Names (A*B) := λ p, names (p.1) ∪ names (p.2).
 Canonical Structure lnamesC := leibnizC lnames.
@@ -129,6 +162,112 @@ Proof.
   rewrite lookup_delete_Some in mtx * => [[_ ?]]; done.
 Qed.
 
+Lemma elem_of_names_env_insert' x τ (Γ: env) ξ:
+  ξ ∈ names (insert' x τ Γ) → ξ ∈ names τ ∨ ξ ∈ names Γ.
+Proof.
+  destruct x; last apply elem_of_names_env_insert_gen.
+  auto.
+Qed.
+
+Inductive heap_wf: lnames → hexpr → Prop :=
+| wf_emp Ξ: heap_wf Ξ hemp
+| wf_star Ξ η₁ η₂ (disj: res_names η₁ ⊥ res_names η₂):
+    heap_wf Ξ η₁ → heap_wf Ξ η₂ → heap_wf Ξ (η₁ ⊗ η₂)
+| wf_pt Ξ ξ τ (inξ: ξ ∈ Ξ) (sub: names τ ⊆ Ξ): heap_wf Ξ (ξ ↦ τ)
+| wf_wait Ξ ξ A η (inξ: ξ ∈ Ξ) (notinξ: ξ ∉ names η)
+          (disj: Ξ ⊥ A):
+    heap_wf (Ξ ∪ A) η → heap_wf Ξ (hwait ξ A η).
+
+Lemma heap_wf_star Ξ η₁ η₂:
+  heap_wf Ξ (η₁ ⊗ η₂) ↔ heap_wf Ξ η₁ ∧ heap_wf Ξ η₂ ∧ res_names η₁ ⊥ res_names η₂.
+Proof.
+  split.
+  - inversion_clear 1; auto.
+  - by intros [?[??]]; constructor.
+Qed.
+
+Lemma heap_wf_wait Ξ ξ A η:
+  heap_wf Ξ (hwait ξ A η) ↔ ξ ∈ Ξ ∧ ξ ∉ names η ∧ Ξ ⊥ A ∧ heap_wf (Ξ ∪ A) η.
+Proof.
+  split.
+  - inversion_clear 1; auto.
+  - by intros [?[?[??]]]; constructor.
+Qed.
+
+Instance heap_wf_proper: Proper ((≡) ==> (≡) ==> iff) heap_wf.
+Proof.
+  intros Ξ ? <-%leibniz_equiv.
+  intros η η' eqη; revert Ξ.
+  induction eqη as [η|η₁ η₂ eqη|η₁ η₂ η₃ eq₁₂ IH₁₂ eq₂₃ IH₂₃|η₁ η₁' eqη₁ IHη₁ η₂ η₂' eqη₂ IHη₂
+                    |ξ A η η' eqη IH|η₁ η₂ η₃|η₁ η₂|η];
+    intro.
+  - done.
+  - done.
+  - by rewrite IH₁₂.
+  - by rewrite !heap_wf_star IHη₁ IHη₂ eqη₁ eqη₂.
+  - by rewrite !heap_wf_wait IH eqη.
+  - rewrite !heap_wf_star; cbn.
+    rewrite disjoint_union_r disjoint_union_l.
+    tauto.
+  - rewrite !heap_wf_star.
+    intuition.
+  - rewrite heap_wf_star.
+    intuition.
+    + constructor.
+    + apply disjoint_empty_l.
+Qed.
+
+(* TODO - figure out how to get a nice notation working. *)
+Inductive typing: lnames → env → expr → hexpr → lnames → type → hexpr → Prop :=
+| tytrue U Γ: typing U Γ Ctrue ∅ ∅ Bool ∅
+| tyfalse U Γ: typing U Γ Cfalse ∅ ∅ Bool ∅
+| tyunit  U Γ: typing U Γ Cunit ∅ ∅ Unit ∅
+| tyvar U Γ (x: string) τ (Γx: Γ !! x = Some τ): typing U Γ x ∅ ∅ τ ∅
+| tylet U Γ (x: binder) η₁ η₂ η₃ τ₁ τ₂ A₁ A₂ e₁ e₂:
+    typing U Γ e₁ η₁ A₁ τ₁ η₂ →
+    typing (U ∪ A₁) (insert' x τ₁ Γ) e₂ η₂ A₂ τ₂ η₃ →
+    typing U Γ (Let x e₁ e₂) η₁ (A₁ ∪ A₂) τ₂ η₃
+| tyif U Γ η₁ η₂ η₃ τ A₁ A₂ e₁ e₂ e₃:
+    typing U Γ e₁ η₁ A₁ tbool η₂ →
+    typing (U ∪ A₁) Γ e₂ η₂ A₂ τ η₃ →
+    typing (U ∪ A₁) Γ e₃ η₂ A₂ τ η₃ →
+    typing U Γ (If e₁ e₂ e₃) η₁ (A₁ ∪ A₂) τ η₃              
+| tyref U Γ e η₁ η₂ τ A ξ (ξ_fresh: ξ ∉ U ∪ A) (post_wf: heap_wf (U ∪ A ∪ {[ξ]}) (η₂ ⊗ ξ ↦ τ)):
+    typing U Γ e η₁ A τ η₂ →
+    typing U Γ (Alloc e) η₁ (A ∪ {[ ξ ]}) (Ref(ξ)) (η₂ ⊗ ξ ↦ τ)
+| tyread U Γ e η₁ η₂ ξ τ A:
+    typing U Γ e η₁ A (Ref(ξ)) (η₂ ⊗ ξ ↦ τ) →
+    typing U Γ (Read e) η₁ A τ (η₂ ⊗ ξ ↦ τ)
+| tywrite U Γ e e' η₁ η₂ η₃ ξ τ A₁ A₂:
+    typing U Γ e η₁ A₁ (Ref(ξ)) η₂ →
+    typing (U ∪ A₁) Γ e' η₂ A₂ τ (η₃ ⊗ ξ ↦ τ) →
+    typing U Γ (Write e e') η₁ (A₁ ∪ A₂) Unit (η₃ ⊗ ξ ↦ τ)
+| typost U Γ e η₁ η₂ τ A ξ (ξ_fresh: ξ ∉ U ∪ A) (wf_post: heap_wf (U ∪ {[ξ]}) (Wait(ξ,A) η₂)):
+    typing U Γ e η₁ A τ η₂ →
+    typing U Γ (Post e) η₁ {[ξ]} (Promise(ξ,A) τ) (Wait(ξ,A) η₂)
+| tywait U Γ e (η₁ η₂ η₃: hexpr) τ ξ A₁ A₂ (wfη: heap_wf (U ∪ A₁ ∪ A₂) (η₂ ⊗ η₃)) (disj: A₂ ⊥ U)
+         (ξ_not_in_τ: ξ ∉ names τ) (ξ_not_in_η₃: ξ ∉ names η₃):
+    typing U Γ e η₁ A₁ (ttask ξ A₂ τ) (η₂ ⊗ hwait ξ A₂ η₃) →
+    typing U Γ (Wait e) η₁ (A₁ ∪ A₂) τ (η₂ ⊗ η₃)         
+| tyframe U Γ e (η₁ η₂: hexpr) τ A (ηf: hexpr)
+          (disjη: res_names η₁ ⊥ res_names ηf)
+          (disjη': res_names η₂ ⊥ res_names ηf)
+          (disjA: A ⊥ names ηf) (wf: heap_wf (U ∪ A) ηf):
+    typing U Γ e η₁ A τ η₂ →
+    typing U Γ e (η₁ ⊗ ηf) A τ (η₂ ⊗ ηf)
+| tyweaken U Γ e η₁ η₂ τ A U' Γ' A' (env_good: names Γ ⊆ U) (pre_good: names η₁ ⊆ U) (disjUA: U' ⊥ A')
+           (subU: U ⊆ U') (subΓ: Γ ⊆ Γ') (subA: A ⊆ A') (wf: heap_wf (A' ∪ U') η₂):
+    typing U Γ e η₁ A τ η₂ →
+    typing U' Γ' e η₁ A' τ η₂
+| typroper U U' Γ e η₁ η₁' A A' τ η₂ η₂'
+           (eqU: U ≡ U') (eqη₁: η₁ ≡ η₁') (eqA: A ≡ A') (eqη₂: η₂ ≡ η₂'):
+    typing U Γ e η₁ A τ η₂ → typing U' Γ e η₁' A' τ η₂'.
+Instance: Proper ((≡) ==> (=) ==> (=) ==> (≡) ==> (≡) ==> (=) ==> (≡) ==> iff) typing.
+Proof.
+  intros U ? <-%leibniz_equiv Γ ? <- e ? <- η₁ η₁' eqη₁ A ? <-%leibniz_equiv τ ? <- η₂ η₂' eqη₂.
+  split; apply typroper; done.
+Qed.
+
 Lemma lookup_insert' {A} x b y z (m: gmap string A):
   insert' b x m !! y = Some z ↔ (b = BNamed y ∧ x = z) ∨ (b ≠ BNamed y ∧ m!!y = Some z).
 Proof.
@@ -145,25 +284,119 @@ Lemma typing_good_names U Γ e η τ η' A:
   names Γ ⊆ U → names η ⊆ U →
   A ⊥ U ∧ names τ ⊆ U ∪ A ∧ names η' ⊆ U ∪ A.
 Proof.
-  induction 1; intros env_good pre_good; cbn -[union].
-  1,2,3: repeat split; set_solver.
-  all: try (destruct IHtyping; auto; set_solver).
-  - repeat split.
-    1,3: set_solver.
+  induction 1; intros env_good' pre_good'; cbn -[union].
+  1,2,3: repeat split; try apply disjoint_empty_l; try apply empty_subseteq.
+  - split; first apply disjoint_empty_l.
+    split; last apply empty_subseteq.
     rewrite right_id.
-    trans (names Γ); last done.
-    intro; rewrite elem_of_names_env; eauto.
-  - destruct IHtyping1 as [disj1 [ty1 post1]]; auto.
-    destruct IHtyping2 as [disj2 [ty2 post2]]; auto.
-    { destruct x; cbn.
-      - trans U; auto; apply union_subseteq_l.
-      - trans (names τ₁ ∪ names Γ).
-        + intro; rewrite elem_of_union; apply elem_of_names_env_insert_gen.
-        + apply union_least; auto.
-          trans U; auto; apply union_subseteq_l. }
-    set_solver.
-  - destruct IHtyping1 as [disj1 [ty1 post1]]; auto.
-    destruct IHtyping2 as [disj2 [ty2 post2]]; auto.
-    { etrans; first done; apply union_subseteq_l. }
-    set_solver.
+    etrans; last apply env_good'.
+    intro ξ.
+    rewrite elem_of_names_env.
+    exists x,τ; auto.
+  - destruct IHtyping1 as [disj₁ [subτ₁ subη₂]]; auto.
+    destruct IHtyping2 as [[disj₂ disjA]%disjoint_union_r [subτ₂ subη₃]]; auto.
+    { intros ξ [?|?]%elem_of_names_env_insert'; auto.
+      apply elem_of_union_l; auto. }
+    rewrite !assoc disjoint_union_l; auto.
+  - destruct IHtyping1 as [disj₁ [subτ₁ subη₂]]; auto.
+    destruct IHtyping2 as [[disj₂ disjA]%disjoint_union_r [subτ₂ subη₃]]; auto.
+    { etrans; first done. apply union_subseteq_l. }
+    rewrite !assoc disjoint_union_l; auto.
+  - destruct IHtyping as [disj [subτ subη']]; auto.
+    rewrite not_elem_of_union in ξ_fresh * => [[??]].
+    repeat split.
+    + rewrite disjoint_union_l disjoint_singleton_l; auto.
+    + rewrite assoc; apply union_subseteq_r.
+    + rewrite (comm (∪) {[ξ]}) !assoc; apply union_mono; last done.
+      apply union_least; done.
+  - destruct IHtyping as [disj [subτ subη']]; auto.
+    repeat split; auto.
+    etrans; last apply subη'.
+    etrans; last apply union_subseteq_r.
+    apply union_subseteq_r.
+  - destruct IHtyping1 as [disj [subτ subη']]; auto.
+    destruct IHtyping2 as [disj' [subτ' subη'']]; auto.
+    { by etrans; last apply union_subseteq_l. }
+    rewrite disjoint_union_r in disj' * => [[??]].
+    rewrite disjoint_union_l; split; auto.
+    split.
+    { apply empty_subseteq. }
+    rewrite (assoc (∪) U); done.
+  - destruct IHtyping as [disj₁ [subτ₁ subη₂]]; auto.
+    rewrite not_elem_of_union in ξ_fresh * => [[??]].
+    rewrite disjoint_singleton_l.
+    split; auto.
+    split; (rewrite comm; apply union_mono; last done).
+    + clear -subτ₁; set_solver.
+    + clear -subη₂; set_solver.
+  - destruct IHtyping as [disj' [subτ subη]]; auto.
+    rewrite disjoint_union_l.
+    rewrite !assoc.
+    repeat split; auto.
+    + intros ξ' inξ'.
+      rewrite elem_of_union.
+      destruct (decide (ξ' ∈ A₂)); auto.
+      left; apply subτ.
+      rewrite /= elem_of_union elem_of_difference; auto.
+    + apply union_least.
+      * etrans; last apply union_subseteq_l.
+        etrans; last apply subη.
+        apply union_subseteq_l.
+      * intros ξ' inξ'.
+        rewrite elem_of_union.
+        destruct (decide (ξ' ∈ A₂)); auto.
+        left; apply subη.
+        cbn -[union].
+        do 2 apply elem_of_union_r.
+        rewrite elem_of_difference; auto.
+  - destruct IHtyping as [disj [subτ subη]]; auto.
+    + etrans; last apply pre_good'.
+      apply union_subseteq_l.
+    + repeat split; auto.
+      apply union_least; auto.
+      trans U; last apply union_subseteq_l.
+      etrans; last apply pre_good'.
+      apply union_subseteq_r.
+  - destruct IHtyping as [disj [namesτ namesη']]; auto.
+    repeat split; auto.
+    + etrans; first apply namesτ.
+      apply union_mono; done.
+    + etrans; first apply namesη'.
+      apply union_mono; done.
+  - subst.
+    apply leibniz_equiv in eqU; subst.
+    apply leibniz_equiv in eqA; subst.
+    rewrite -eqη₂.
+    destruct IHtyping as [? [??]]; auto.
+    rewrite eqη₁; done.
+Qed.
+
+Lemma heap_wf_names U η: heap_wf U η → names η ⊆ U.
+Proof.
+  induction 1; cbn -[union].
+  - apply empty_subseteq.
+  - by apply union_least.
+  - apply union_least; auto.
+    apply elem_of_subseteq_singleton; done.
+  - apply union_least.
+    + by apply elem_of_subseteq_singleton.
+    + clear -IHheap_wf.
+      set_solver.
+Qed.
+
+Lemma typing_wf  U Γ e η τ η' A:
+  typing U Γ e η A τ η' → heap_wf U η → heap_wf (U ∪ A) η'.
+Proof.
+  induction 1; intro wf'.
+  1-4: constructor.
+  all: try by rewrite ?union_assoc_L; auto.
+  - inversion_clear wf'.
+    constructor; auto.
+  - by rewrite union_comm_L.
+  - apply leibniz_equiv in eqU.
+    apply leibniz_equiv in eqA.
+    subst.
+    rewrite -eqη₂.
+    apply IHtyping.
+    rewrite eqη₁; done.
 Qed.
