theories/closure.v
@@ -1,6 +1,6 @@
 From iris.proofmode Require Import tactics.
 From esop Require Import closed_async closed_basic closed_memory closed_meta delayed types
-     typetranslation corecalculus.
+     typetranslation corecalculus exprfacts stringfresh.
 From iris.base_logic.lib Require Import invariants.
 From stdpp Require Import gmap.
 
@@ -16,8 +16,8 @@ Section FullClosure.
     iApply (closed_strengthen ∅).
     5: iApply closed_true.
     1,2: constructor.
-    - by rewrite map_subseteq_spec => [??]; rewrite lookup_empty => [?].
-    - done.
+    2: apply empty_subseteq.
+    rewrite map_subseteq_spec => [??]; rewrite lookup_empty => [?]; done.
   Qed.
   
   Lemma closure_false: delayed_simulation U Γ ∅ Cfalse Cfalse ∅ Bool ∅.
@@ -59,19 +59,553 @@ Section FullClosure.
     intros [[<- <-]|[_ [=]]]; done.
   Qed.
 
+  Lemma subst_empty e: subst ∅ e = e.
+  Proof.
+    induction e; rewrite /=; try congruence.
+    - by rewrite lookup_empty.
+    - f_equal.
+      assert (∀ b, delete' b (∅: gmap string expr) = ∅) as red.
+      { destruct b; first done.
+        apply delete_empty. }
+      rewrite !red IHe //.
+  Qed.
+
+  Lemma dom_insert' {A} b (x: A) m: dom (gset string) (insert' b x m) = {[?b]} ∪ dom _ m.
+  Proof.
+    apply leibniz_equiv.
+    destruct b.
+    - rewrite /= left_id //.
+    - rewrite /= dom_insert //.
+  Qed.
+
+  Lemma type_var_string U' (Γ': env) x τ (val_x: Γ' !! x = Some τ) (η: hexpr) (wf: heap_wf U' η):
+    typing U' Γ' x η ∅ τ η.
+  Proof.
+    rewrite -(left_id hemp hstar η).
+    apply tyframe.
+    1-3: apply disjoint_empty_l.
+    2: by constructor.
+    rewrite union_empty_r_L; done.
+  Qed.
+
+  Lemma names_env_insert Γ' x τ: names (<[x:=τ]> Γ') ⊆ names τ ∪ names Γ'.
+  Proof.
+    intro ξ.
+    rewrite elem_of_union !elem_of_names_env.
+    intros [x' [τ' [[[??]|[??]]%lookup_insert_Some inξ]]]; subst; eauto.
+  Qed.
+  
+  Lemma good_after_bind {e η A τ η' y}:
+    names η ⊆ U →
+    typing U Γ e η A τ η' →
+    names (<[y:=τ]>Γ) ∪ names η' ⊆ U ∪ A.
+  Proof.
+    intros subη [disj [subτ subη']]%typing_good_names; auto.
+    pose proof (names_env_insert Γ y τ) as sub.
+    clear -sub subη' subτ good_env.
+    set_solver.
+  Qed.
+  
   Lemma closure_let (x: binder) η₁ η₂ η₃ τ₁ τ₂ A₁ A₂ e₁ e₂ e₁' e₂':
+    heap_wf U η₁ →
     delayed_simulation U Γ η₁ e₁ e₁' A₁ τ₁ η₂ →
     delayed_simulation (U ∪ A₁) (insert' x τ₁ Γ) η₂ e₂ e₂' A₂ τ₂ η₃ →
     delayed_simulation U Γ η₁ (Let x e₁ e₂) (Let x e₁' e₂') (A₁ ∪ A₂) τ₂ η₃.
   Proof.
-    intros [good₁ ty₁ ty₁' del₁] [good₂ ty₂ ty₂' del₂].
+    intros wf [good₁ ty₁ ty₁' del₁] [good₂ ty₂ ty₂' del₂].
+    assert (typing U Γ (Let x e₁ e₂) η₁ (A₁ ∪ A₂) τ₂ η₃) as ty_let.
+    { econstructor; eauto. }
+    assert (typing U Γ (Let x e₁' e₂') η₁ (A₁ ∪ A₂) τ₂ η₃) as ty_let'.
+    { econstructor; eauto. }
     split.
-    - done.
-    - by econstructor.
-    - by econstructor.
-    - destruct x as [|x].
-      + admit.
-      + iPoseProof (delayed_bind $! x e₁ e₁' [CAppR
+    1-3: done.
+    set (y := fresh (dom (gset string) Γ)).
+    assert (∀ (e': expr) z, z ∈ dom (gset string) (insert' x τ₁ Γ) →
+                            delete' x (<[y:=e']>∅) !! z = None).
+    { intros *.
+      rewrite dom_insert' elem_of_union elem_of_singleton' => [[<-|inz]].
+      - rewrite /= lookup_delete //.
+      - rewrite lookup_delete'_None lookup_insert_ne ?lookup_empty; first auto.
+        intros <-.
+        apply is_fresh in inz; done. }
+    iApply (delayed_bind_strong y e₁ e₁'
+                                [EAppR (Rec BAnon x e₂)]
+                                [EAppR (Rec BAnon x e₂')]
+                                Γ τ₁ τ₂ η₁ η₂ η₃ U A₁ A₂).
+    1,2: intro; rewrite /= (subst_closed (dom _ (insert' x τ₁ Γ))) //.
+    1,3: by eapply typing_closed.
+    1,2: auto.
+    1,2: repeat constructor; rewrite /= left_id -(dom_insert' x τ₁ Γ); by eapply typing_closed.
+    1: by split.
+    rewrite -(union_empty_l_L A₂).
+    assert (∀ e, typing (U ∪ A₁) (insert' x τ₁ Γ) e η₂ A₂ τ₂ η₃ →
+                 typing (U ∪ A₁ ∪ ∅) (insert' x τ₁ (<[y:=τ₁]>Γ)) e η₂ A₂ τ₂ η₃).
+    { intro.
+      apply typing_good_names in ty₁.
+      2,3: clear -good₁; set_solver.
+      destruct ty₁ as [disj₁ [subτ₁ subη₂]].
+      assert (names (insert' x τ₁ Γ) ⊆ U ∪ A₁).
+      { intro ξ; rewrite elem_of_names_env => [[x' [τ' [mt inξ]]]].
+        rewrite lookup_insert' in mt * => [[[? ?]|[neq mt]]]; subst; first auto.
+        rewrite elem_of_union; left.
+        apply good₁, elem_of_union; left.
+        rewrite elem_of_names_env; eauto. }
+      apply typing_good_names in ty₂; auto.
+      destruct ty₂ as [[??]%disjoint_union_r [??]].
+      apply tyweaken.
+      1,2,6: done.
+      2: rewrite right_id; done.
+      1: rewrite right_id; apply disjoint_union_l; split; auto.
+      2: rewrite union_empty_r_L union_comm_L.
+      2: eapply typing_wf; first done.
+      2: by eapply typing_wf.
+      apply map_subseteq_spec.
+      intros x' τ'.
+      rewrite !lookup_insert'.
+      intros [case|[neq lookup]]; auto.
+      right; split; trivial.
+      rewrite lookup_insert_ne //.
+      intros <-.
+      apply (elem_of_dom_2 (D:=gset string)) in lookup.
+      apply is_fresh in lookup; done. }
+    split.
+    2,3: eapply tylet; auto.
+    2,3: apply type_var_string; first apply lookup_insert.
+    2,3: by eapply typing_wf.
+    { eapply good_after_bind; eauto.
+      clear -good₁; set_solver. }
+    destruct x.
+    - iApply closed_let_anon; first apply lookup_insert.
+      rewrite union_empty_l_L.
+      iApply closed_strengthen.
+      5: iApply del₂.
+      1,2,4: done.
+      apply map_subseteq_spec.
+      intros x' τ' mt.
+      rewrite lookup_insert_ne; first done.
+      intros <-.
+      apply (elem_of_dom_2 (D:=gset string)), is_fresh in mt; done.
+    - iApply closed_let; first apply lookup_insert.
+      rewrite union_empty_l_L.
+      iApply closed_strengthen.
+      5: iApply del₂.
+      1,2,4: done.
+      apply map_subseteq_spec.
+      intros x' τ' mt.
+      rewrite lookup_insert' in mt * => [[[eqx <-]|[neqx mt]]].
+      + injection eqx as <-; apply lookup_insert.
+      + rewrite lookup_insert_ne; last congruence.
+        rewrite lookup_insert_ne; first done.
+        intros <-.
+        apply (elem_of_dom_2 (D:=gset string)), is_fresh in mt; done.
+  Qed.
+
+  Lemma ext_env_with_fresh (Γ': env) τ: Γ' ⊆ <[fresh (dom (gset string) Γ') := τ]>Γ'.
+  Proof.
+    apply insert_subseteq.
+    rewrite -(not_elem_of_dom (D:=gset string)).
+    apply is_fresh.
+  Qed.
+  
+  Lemma closure_if η₁ η₂ η₃ τ A₁ A₂ e₁ e₁' e₂ e₂' e₃ e₃':
+    heap_wf U η₁ →
+    delayed_simulation U Γ η₁ e₁ e₁' A₁ tbool η₂ →
+    delayed_simulation (U ∪ A₁) Γ η₂ e₂ e₂' A₂ τ η₃ →
+    delayed_simulation (U ∪ A₁) Γ η₂ e₃ e₃' A₂ τ η₃ →
+    delayed_simulation U Γ η₁ (If e₁ e₂ e₃) (If e₁' e₂' e₃') (A₁ ∪ A₂) τ η₃.
+  Proof.
+    intros wf [good₁ ty₁ ty₁' del₁] [good₂ ty₂ ty₂' del₂] [good₃ ty₃ ty₃' del₃].
+    assert (names η₁ ⊆ U).
+    { etrans; last done. apply union_subseteq_r. }
+    destruct (typing_good_names _ _ _ _ _ _ _ ty₁) as [disj₁ [subτ₁ subη₂]].
+    1,2: done.
+    destruct (typing_good_names _ _ _ _ _ _ _ ty₂) as [disj₂ [subτ₂ subη₃]].
+    { trans U; first done. apply union_subseteq_l. }
+    { done. }
+    split; first done.
+    1,2: by econstructor.
+    set (x:=fresh (dom (gset string) Γ)).
+    iApply (delayed_bind x e₁ e₁' [CIf e₂ e₃] [CIf e₂' e₃'] Γ tbool τ η₁ η₂ η₃ U A₁ A₂).
+    1,2: intro; rewrite /= !(subst_closed (dom _ Γ)) //.
+    1,3,5,7: by eapply typing_closed.
+    1,2,3,4: intros y iny; rewrite lookup_insert_ne ?lookup_empty //.
+    1,2,3,4: intros <-; by apply is_fresh in iny.
+    - by split.
+    - split.
+      + eapply good_after_bind; eauto.
+      + cbn.
+        rewrite -(union_empty_l_L A₂).
+        apply tyif with (η₂ := η₂).
+        { apply type_var_string; first apply lookup_insert. by eapply typing_wf. }
+        all: rewrite union_empty_r_L.
+        all: eapply (tyweaken (U ∪ A₁) Γ); try done.
+        3,6: rewrite union_comm_L.
+        3,4: eapply typing_wf; first done.
+        3,4: by eapply typing_wf.
+        2,4: apply ext_env_with_fresh.
+        all: etrans; first done.
+        all: apply union_subseteq_l.
+      + cbn.
+        rewrite -(union_empty_l_L A₂).
+        apply tyif with (η₂ := η₂).
+        { apply type_var_string; first apply lookup_insert. by eapply typing_wf. }
+        all: rewrite union_empty_r_L.
+        all: eapply (tyweaken (U ∪ A₁) Γ); try done.
+        3,6: rewrite union_comm_L.
+        3,4: eapply typing_wf; first done.
+        3,4: by eapply typing_wf.
+        2,4: apply ext_env_with_fresh.
+        all: etrans; first done.
+        all: apply union_subseteq_l.
+      + iApply closed_if.
+        * apply lookup_insert.
+        * iApply closed_strengthen; last iApply del₂.
+          all: try done.
+          apply ext_env_with_fresh.
+        * iApply closed_strengthen; last iApply del₃.
+          all: try done.
+          apply ext_env_with_fresh.
+  Qed.
+
+  Lemma strengthen_heap_wf Ξ η: heap_wf Ξ η → ∀ Ξ', Ξ' ⊆ Ξ → names η ⊆ Ξ' → heap_wf Ξ' η.
+  Proof.
+    induction 1; intros; constructor; auto.
+    - apply IHheap_wf1; auto.
+      etrans; last done.
+      apply union_subseteq_l.
+    - apply IHheap_wf2; auto.
+      etrans; last done.
+      apply union_subseteq_r.
+    - by apply H1, elem_of_union, or_introl, elem_of_singleton.
+    - etrans; last done.
+      apply union_subseteq_r.
+    - by apply H2, elem_of_union, or_introl, elem_of_singleton.
+    - by intros ? ?%H1; apply disj.
+    - apply IHheap_wf.
+      + by apply union_mono.
+      + cbn -[union] in H2.
+        clear -H2.
+        intros ξ' inξ'.
+        rewrite elem_of_union.
+        destruct (decide (ξ' ∈ A)) as [case|case]; auto.
+        left; apply H2.
+        rewrite elem_of_union elem_of_difference; auto.
+  Qed.
+  
+      
+  Lemma closure_ref e e' η₁ η₂ τ A ξ (ξ_fresh: ξ ∉ U ∪ A) (wf: heap_wf (U ∪ A ∪ {[ξ]}) (η₂ ⊗ ξ ↦ τ)):
+    delayed_simulation U Γ η₁ e e' A τ η₂ →
+    delayed_simulation U Γ η₁ (Alloc e) (Alloc e') (A ∪ {[ ξ ]}) (Ref(ξ)) (η₂ ⊗ ξ ↦ τ).
+  Proof.
+    intros [good tye tye' del].
+    split.
+    1: done.
+    1,2: by constructor.
+    set (x := fresh (dom (gset string) Γ)).
+    iApply (delayed_bind x e e' [CAlloc] [CAlloc] Γ τ (Ref(ξ)) η₁ η₂ (η₂ ⊗ ξ ↦ τ)).
+    1,2: done.
+    1: by split.
+    destruct (typing_good_names _ _ _ _ _ _ _ tye) as [disj [subτ subη₂]].
+    1,2: clear -good; set_solver.
+    assert (typing (U ∪ A) (<[x:=τ]>∅) (Alloc x) η₂ {[ξ]} (Ref(ξ)) (η₂ ⊗ ξ ↦ τ)).
+    { rewrite -(union_empty_l_L {[ξ]}).
+      constructor; first by rewrite union_empty_r.
+      { by rewrite union_empty_r_L. }
+      rewrite -(left_id hemp hstar η₂).
+      apply tyframe.
+      1-3: apply disjoint_empty_l.
+      2: constructor; apply lookup_insert.
+      inversion_clear wf as [|??? _ wf' _| |].
+      rewrite union_empty_r_L.
+      eapply strengthen_heap_wf; try done.
+      apply union_subseteq_l. }
+    assert (typing (U ∪ A) (<[x:=τ]>Γ) (Alloc x) η₂ {[ξ]} (Ref(ξ)) (η₂ ⊗ ξ ↦ τ)).
+    { eapply tyweaken; last done.
+      2,4,6: done.
+      2: by rewrite disjoint_singleton_r.
+      - intros ξ'.
+        rewrite elem_of_names_env => [[x' [τ' [mt inξ']]]].
+        rewrite lookup_insert_Some in mt * => [[[??]|[? contra]]].
+        + subst; auto.
+        + by apply lookup_empty_Some in contra.
+      - apply insert_mono, map_subseteq_spec.
+        intros ?? []%lookup_empty_Some.
+      - by rewrite union_comm_L. }
+    split.
+    2,3: done.
+    { eapply good_after_bind; eauto.
+      etrans; last done.
+      apply union_subseteq_r. }
+    rewrite comm -{1}(left_id hemp hstar η₂).
+    iApply closed_frame.
+    { cbn; apply disjoint_singleton_l.
+      contradict ξ_fresh.
+      apply subη₂, res_names_sub_names, ξ_fresh. }
+    { apply disjoint_empty_l. }
+    { apply disjoint_singleton_r.
+      contradict ξ_fresh.
+      apply subη₂, ξ_fresh. }
+    iApply (closed_strengthen (U ∪ A) (<[x:=τ]>∅)).
+    4: done.
+    1,2: rewrite -(left_id hemp hstar (hpt ξ τ)).
+    1,2: rewrite -(union_empty_l_L {[ξ]}).
+    1,2: apply tyref.
+    1,4: by rewrite union_empty_r_L.
+    2,4: apply type_var_string; last constructor.
+    2,3: apply lookup_insert.
+    1,2: rewrite left_id.
+    1,2: constructor.
+    1,3: by apply elem_of_union_r, elem_of_singleton.
+    1,2: rewrite right_id.
+    1,2: etrans; first done.
+    1,2: apply union_subseteq_l.
+    { apply insert_mono, map_subseteq_spec.
+      intros ?? []%lookup_empty_Some. }
+    iApply closed_alloc.
+    contradict ξ_fresh; auto.
+  Qed.
+
+  Lemma closure_read e e' η₁ η₂ ξ τ A:
+    heap_wf U η₁ →
+    delayed_simulation U Γ η₁ e e' A (Ref(ξ)) (η₂ ⊗ ξ ↦ τ) →
+    delayed_simulation U Γ η₁ (Read e) (Read e') A τ (η₂ ⊗ ξ ↦ τ).
+  Proof.
+    intros wf [good ty ty' del].
+    split; first done.
+    1,2: by constructor.
+    set (x := fresh (dom (gset string) Γ)).
+    rewrite -(union_empty_r_L A).
+    iApply (delayed_bind x e e' [CRead] [CRead] Γ (Ref(ξ)) τ).
+    1,2: done.
+    { by split. }
+    split.
+    { eapply good_after_bind; last done.
+      etrans; last apply good.
+      apply union_subseteq_r. }
+    1,2: constructor; apply type_var_string; first apply lookup_insert.
+    1,2: by eapply typing_wf.
+    iApply (closed_strengthen (U ∪ A) (<[x:=tref ξ]>∅)).
+    4: done.
+    1,2: constructor; apply type_var_string; first apply lookup_insert.
+    1,2: by eapply typing_wf.
+    { apply insert_mono, map_subseteq_spec.
+      intros ?? []%lookup_empty_Some. }
+    rewrite comm.
+    apply typing_wf in ty; auto.
+    inversion_clear ty.
+    iApply closed_frame.
+    1,2: done.
+    { apply disjoint_empty_r. }
+    iApply closed_read.
+  Qed.
+
+  Lemma closure_write e₁ e₁' e₂ e₂' η₁ η₂ η₃ ξ τ A₁ A₂:
+    heap_wf U η₁ →
+    delayed_simulation U Γ η₁ e₁ e₁' A₁ (Ref(ξ)) η₂ →
+    delayed_simulation (U ∪ A₁) Γ η₂ e₂ e₂' A₂ τ (η₃ ⊗ ξ ↦ τ) →
+    delayed_simulation U Γ η₁ (Write e₁ e₂) (Write e₁' e₂') (A₁ ∪ A₂) tunit (η₃ ⊗ ξ ↦ τ).
+  Proof.
+    intros wf [good₁ ty₁ ty₁' del₁] [good₂ ty₂ ty₂' del₂].
+    split; first done.
+    1,2: by econstructor.
+    set (x := fresh (dom (gset string) Γ)).
+    iApply (delayed_bind x e₁ e₁' [CWriteL e₂] [CWriteL e₂']).
+    1,2: intro; cbn; do 2 f_equal; apply (subst_closed (dom _ Γ)).
+    1,3: by eapply typing_closed.
+    1,2: intros y iny; rewrite lookup_insert_None lookup_empty; split; auto.
+    1,2: by intros <-; apply is_fresh in iny.
+    1: by split.
+    cbn.
+    apply typing_good_names in ty₁'; auto.
+    2: etrans; last done; apply union_subseteq_r.
+    destruct ty₁' as [disj₁ [inξ subη₂]].
+    destruct (typing_good_names _ _ _ _ _ _ _ ty₂) as [[disj₂ disj₂']%disjoint_union_r [_ subη₃]].
+    { etrans; first done. apply union_subseteq_l. }
+    { done. }
+    split.
+    { apply union_least; auto.
+      etrans; first apply names_env_insert.
+      apply union_least; auto.
+      etrans; first done.
+      apply union_subseteq_l. }
+    1-3: rewrite -(union_empty_l_L A₂).
+    1,2: econstructor.
+    1,3: apply type_var_string; first apply lookup_insert.
+    1,2: by eapply typing_wf.
+    1,2: rewrite union_empty_r_L.
+    1,2: eapply tyweaken; last done.
+    1,8: etrans; first done; apply union_subseteq_l.
+    1,3,5,7,9,11: done.
+    1,4: apply disjoint_union_l; auto.
+    1,3: apply insert_subseteq, (not_elem_of_dom (D:=gset string)), is_fresh.
+    1,2: rewrite union_comm_L; eapply typing_wf; first done.
+    1,2: by eapply typing_wf.
+    rewrite union_comm_L.
+    set (y := fresh (dom (gset string) (<[x:=tref ξ]>Γ))).
+    assert (y ≠ x).
+    { intros eqxy; subst y.
+      pose proof (is_fresh (dom (gset string) (<[x:=tref ξ]>Γ))) as contra.
+      rewrite eqxy dom_insert not_elem_of_union not_elem_of_singleton in contra *.
+      tauto. }
+    iApply (delayed_bind_strong y e₂ e₂' [EWriteR x] [EWriteR x] (<[x:=tref ξ]>Γ) τ tunit
+                                η₂ (η₃ ⊗ ξ ↦ τ) (η₃ ⊗ ξ ↦ τ) (U ∪ A₁) A₂ ∅).
+    1,2: intro; rewrite /= lookup_insert_ne //.
+    1,2: repeat constructor.
+    1,2: rewrite dom_insert elem_of_union elem_of_singleton; auto.
+    { split.
+      2,3: apply tyweaken with (U := U ∪ A₁) (Γ := Γ) (A:=A₂); try done.
+      3,7: apply disjoint_union_l; auto.
+      2,5: etrans; first done; apply union_subseteq_l.
+      2,4: apply insert_subseteq, (not_elem_of_dom (D:=gset string)), is_fresh.
+      2,3: rewrite union_comm_L.
+      2,3: eapply typing_wf; try done.
+      2,3: by eapply typing_wf.
+      { apply union_least; auto.
+        etrans; first apply names_env_insert.
+        apply union_least; auto.
+        etrans; first done.
+        apply union_subseteq_l. }
+      iApply closed_strengthen; last iApply del₂.
+      4: done.
+      3: apply insert_subseteq, (not_elem_of_dom (D:=gset string)), is_fresh.
+      1,2: done. }
+    cbn.
+    apply typing_wf in ty₂'; last by eapply typing_wf.
+    inversion_clear ty₂' as [|??? disjξ wfη₃ wfξ| |].
+    assert (typing (U ∪ A₁ ∪ A₂) (<[y:=τ]>(<[x:=tref ξ]>∅)) (Write x y) (ξ ↦ τ) (∅ ∪ ∅) Unit (ξ ↦ τ))
+      as ty.
+    { rewrite -(left_id hemp hstar (hpt ξ τ)).
+      eapply tywrite.
+      - apply type_var_string.
+        + rewrite lookup_insert_ne // lookup_insert //.
+        + by rewrite left_id.
+      - apply type_var_string.
+        + apply lookup_insert.
+        + by rewrite left_id union_empty_r_L. }
+    assert (typing (U ∪ A₁ ∪ A₂) (<[y:=τ]>(<[x:=tref ξ]>Γ)) (Write x y) (ξ ↦ τ) (∅ ∪ ∅) Unit (ξ ↦ τ)).
+    { eapply tyweaken; last done.
+      all: rewrite ?union_empty_l_L; auto.
+      4: apply insert_mono, insert_mono, map_subseteq_spec.
+      4: intros ?? []%lookup_empty_Some.
+      3: apply disjoint_empty_r.
+      2: by eapply heap_wf_names.
+      etrans; first apply names_env_insert.
+      apply union_least; first by inversion_clear wfξ.
+      etrans; first apply names_env_insert.
+      etrans; last apply union_subseteq_l.
+      apply union_least; auto.
+      apply empty_subseteq. }
+    rewrite (comm hstar η₃).
+    split.
+    2,3: rewrite -(union_empty_l_L ∅).
+    2,3: constructor; auto.
+    2,4: rewrite left_id; apply disjoint_empty_l.
+    2,3: by rewrite !union_empty_r_L.
+    { apply union_least.
+      - etrans; first apply (names_env_insert (<[x:=tref ξ]>Γ) y τ).
+        apply union_least.
+        { apply typing_good_names in ty₂; try tauto.
+          etrans; first done. apply union_subseteq_l. }
+        etrans; first apply names_env_insert.
+        etrans; last apply union_subseteq_l.
+        apply union_least; auto.
+        etrans; first done.
+        apply union_subseteq_l.
+      - cbn -[union]; apply union_least.
+        + inversion_clear wfξ.
+          apply union_least; auto.
+          apply elem_of_subseteq_singleton; done.
+        + by apply heap_wf_names. }
+    iApply closed_frame; auto.
+    { apply disjoint_empty_r. }
+    rewrite union_empty_l_L insert_commute // in ty *.
+    iApply (closed_strengthen (U ∪ A₁ ∪ A₂)).
+    1,2,4: done.
+    2: iApply closed_write; auto.
+    rewrite insert_commute //.
+    apply insert_mono, insert_mono, map_subseteq_spec.
+    intros ?? []%lookup_empty_Some.
+  Qed.
+
+  Lemma closure_post e e' η₁ η₂ τ A ξ (ξ_fresh: ξ ∉ U ∪ A) (wf: heap_wf (U ∪ {[ξ]}) (Wait(ξ,A) η₂)):
+    delayed_simulation U Γ η₁ e e' A τ η₂ →
+    delayed_simulation U Γ η₁ (Post e) (Post e') {[ξ]} (Promise(ξ,A) τ) (Wait(ξ,A) η₂).
+  Proof.
+    intros [good tye tye' del].
+    split; auto.
+    1,2: by constructor.
+    rewrite not_elem_of_union in ξ_fresh * => [[notinU notinA]].
+    apply typing_good_names in tye; auto.
+    2: etrans; last done; apply union_subseteq_r.
+    destruct tye as [disj [subτ subη]].
+    iApply closed_post; auto.
+    4: iApply del.
+    - contradict notinU.
+      apply good, elem_of_union_r, notinU.
+    - by intros [?|?]%subτ%elem_of_union.
+    - by intros [?|?]%subη%elem_of_union.
+  Qed.
+
+  Lemma closure_wait e e' (η₁ η₂ η₃: hexpr) (τ: type) ξ A₁ A₂
+        (disjA: A₁ ⊥ A₂) (disjU: U ⊥ A₂) (wf: heap_wf (U ∪ A₁ ∪ A₂) (η₂ ⊗ η₃))
+        (ξ_τ: ξ ∉ names τ) (ξ_η₃: ξ ∉ names η₃):
+    heap_wf U η₁ →
+    delayed_simulation U Γ η₁ e e' A₁ (ttask ξ A₂ τ) (η₂ ⊗ hwait ξ A₂ η₃) →
+    delayed_simulation U Γ η₁ (Wait e) (Wait e') (A₁ ∪ A₂) τ (η₂ ⊗ η₃).
+  Proof.
+    intros wfη₁ [good tye tye' del].
+    split; first done.
+    1,2: econstructor; try done.
+    pose proof (typing_wf _ _ _ _ _ _ _ tye' wfη₁) as wf'.
+    set (x := fresh (dom (gset string) Γ)).
+    iApply (delayed_bind x e e' [CWait] [CWait]).
+    1,2: done.
+    { by split. }
+    split.
+    2,3: rewrite -(union_empty_l_L A₂).
+    2,3: eapply tywait.
+    all: rewrite ?union_empty_r_L ?union_empty_l_L.
+    2,4,5,7,9,10: done.
+    3,5: apply type_var_string; first apply lookup_insert.
+    3,4: done.
+    2,3: apply disjoint_union_r; auto.
+    { apply union_least.
+      - etrans; first apply names_env_insert.
+        apply union_least.
+        2: by etrans; last apply union_subseteq_l.
+        apply typing_good_names in tye; try tauto.
+        by etrans; first apply union_subseteq_r.
+      - apply typing_good_names in tye; try tauto.
+          by etrans; first apply union_subseteq_r. }
+    rewrite !(comm hstar η₂).
+    iApply closed_frame.
+    { by inversion_clear wf. }
+    { apply typing_wf in tye; auto.
+      inversion_clear tye; done. }
+    { apply typing_good_names in tye; auto.
+      2: etrans; last apply good; apply union_subseteq_r.
+      destruct tye as [_ [_ sub]].
+      intros ξ' inξ'.
+      enough (ξ' ∈ U ∪ A₁) as [?|?]%elem_of_union.
+      { by apply disjU. }
+      { by apply disjA. }
+      apply sub, elem_of_union_l, inξ'. }                
+    assert (heap_wf (U ∪ A₁) (Wait(ξ,A₂) η₃)).
+    { apply typing_wf in tye; auto.
+      inversion_clear tye; done. }
+    iApply (closed_strengthen (U ∪ A₁) (<[x:=ttask ξ A₂ τ]>∅)).
+    4: done.
+    1,2: rewrite -(union_empty_l_L A₂).
+    1,2: rewrite -{2}(left_id hemp hstar η₃).
+    1,2: eapply tywait; auto; try done.
+    1,4: rewrite union_empty_r_L !left_id.
+    1,2: by inversion_clear wf.
+    1,3: apply disjoint_union_r; auto.
+    1,2: rewrite union_empty_l_L !left_id.
+    1,2: by apply type_var_string; first apply lookup_insert.
+    { apply insert_mono, map_subseteq_spec.
+      intros ?? []%lookup_empty_Some. }
+    by iApply closed_wait.
   Qed.
   
 End FullClosure.
