theories/delayed.v
@@ -11,6 +11,24 @@ Section Definitions.
   Definition simulation:
     env → expr → hexpr → gset gname → type → hexpr → conn_map → conn_map → iProp Σ
     := simulation_body int_s_type int_s_heap.
+  Global Instance simulation_proper:
+    Proper ((=) ==> (=) ==> (≡) ==> (=) ==> (=) ==> (≡) ==> (=) ==> (=) ==> (≡))
+           simulation.
+  Proof.
+    rewrite /simulation /simulation_body /existential_triple.
+    intros Γ ? <- e ? <- η₁ η₁' eqη₁ A ? <- τ ? <- η₂ η₂' eqη₂ D ? <- D' ? <-.
+    f_equiv; intro N.
+    f_equiv; intro σ.
+    f_equiv; intro p.
+    f_equiv; intro K.
+    do 3 f_equiv.
+    { by apply int_s_heap_proper. }
+    do 2 f_equiv; intro v.
+    do 2 f_equiv; intro d.
+    f_equiv; intro N'.
+    do 2 f_equiv.
+    apply int_s_heap_proper; done.
+  Qed.
   
   Definition delayed_typed Γ η e e' A τ η' :=
     ∀ D N σ,
@@ -20,6 +38,27 @@ Section Definitions.
                             int_i_type τ d' Nᵢ'  xᵢ ∧
                             (□simulation Γ e' η A τ η' D D') ∧
                             int_i_heap η' D' Nᵢ' }}.
+  Global Instance delayed_typed_proper:
+    Proper ((=) ==> (≡) ==> (=) ==> (=) ==> (=) ==> (=) ==> (≡) ==> (⊣⊢))
+           delayed_typed.
+  Proof.
+    intros Γ ? <- η₁ η₁' eqη₁ e ? <- e' ? <- A ? <- τ ? <- η₂ η₂' eqη₂.
+    rewrite /delayed_typed.
+    f_equiv; intro D.
+    f_equiv; intro N.
+    f_equiv; intro σ.
+    f_equiv.
+    { by f_equiv; apply int_i_heap_proper. }
+    apply wp_proper; intro v.
+    f_equiv; intro N'.
+    f_equiv; intro D'.
+    f_equiv; intro d'.
+    do 3 f_equiv.
+    2: by apply int_i_heap_proper.
+    f_equiv.
+    apply simulation_proper; done.
+  Qed.
+  
   Record delayed_simulation U Γ (η: hexpr) e e' A (τ: type) (η': hexpr) :=
     Delayed {
         ds_used_names: names Γ ∪ names η ⊆ U;
@@ -27,9 +66,20 @@ Section Definitions.
         ds_type_e': typing U Γ e' η A τ η';
         ds_sim: delayed_typed Γ η e e' A τ η'
       }.
+  Global Instance delayed_simulation_proper:
+    Proper ((=) ==> (=) ==> (≡) ==> (=) ==> (=) ==> (=) ==> (=) ==> (≡) ==> iff)
+           delayed_simulation.
+  Proof.
+    intros U ? <- Γ ? <- η₁ η₁' eqη₁ e ? <- e' ? <- A ? <- τ ? <- η₂ η₂' eqη₂.
+    revert η₁ η₁' eqη₁ η₂ η₂' eqη₂.
+    apply proper_sym_impl_iff_2.
+    1,2: apply _.
+    intros η₁ η₁' eqη₁ η₂ η₂' eqη₂ [good ty ty' del].
+    split.
+    - by rewrite -eqη₁.
+    - by rewrite -eqη₁ -eqη₂.
+    - by rewrite -eqη₁ -eqη₂.
+    - by rewrite -eqη₁ -eqη₂.
+  Qed.
+  
 End Definitions.
-
-Section Meta.
-  Context `{allG Σ}.
-  Local Open Scope I.
-End Meta.
