theories/stringfresh.v
@@ -1,0 +1,99 @@
+From stdpp Require Import strings gmap fin_collections pretty.
+From mathcomp Require Import ssreflect.
+
+Section General.
+  Context `{FinCollection A C}.
+  Definition set_recursion {B} (f: ∀ c, (∀ c', c' ⊂ c → B) → B) (c: C): B :=
+    Fix collection_wf (const B) f c.
+
+  Lemma set_recursion_unfold {B} (f: ∀ c, (∀ c', c' ⊂ c → B) → B)
+        (f_proper: ∀ x g g', (∀ c' H, g c' H = g' c' H) → f x g = f x g')
+        c:
+    set_recursion f c = f c (λ c' _, set_recursion f c').
+  Proof. rewrite /set_recursion {1}Fix_eq //. Qed.
+
+  Lemma set_recursion_unfold' {B} (eqB: Equiv B) (f: ∀ c, (∀ c', c' ⊂ c → B) → B)
+        (f_proper: ∀ x g g', (∀ c' H, g c' H ≡ g' c' H) → f x g ≡ f x g')
+        c:
+    set_recursion f c ≡ f c (λ c' _, set_recursion f c').
+  Proof.
+    unfold set_recursion, Fix.
+    destruct (collection_wf c); cbn.
+    apply f_proper.
+    intros c' subc.
+    generalize (a c' subc) as acc, (collection_wf c') as acc'.
+    clear c subc a.
+    induction c' as [c IH] using (well_founded_ind collection_wf).
+    intros [acc] [acc']; cbn.
+    apply: f_proper => [c' sub].
+    apply IH, sub.
+  Qed.
+
+  Lemma subset_difference_in {x: A} {s: C} (inx: x ∈ s): s ∖ {[ x ]} ⊂ s.
+  Proof. set_solver. Qed.
+End General.
+
+Section FreshString.
+  Context `{FinCollection string C} `{InDec: ∀ (x: string) (s: C), Decision (x ∈ s)} (prefix: string).
+
+  Definition cand (n: N) := prefix +:+ pretty n.
+  Definition find_fresh_string (s: C) n :=
+    set_recursion (λ (c: C) rec (n: N),
+                   let x := cand n in
+                   match decide (x ∈ c) return string with
+                   | left H => rec (c ∖ {[ x ]}) (subset_difference_in H) (1+n)%N
+                   | right _ => x
+                   end) s n.
+  Lemma find_fresh_string_spec c: ∀ n, ∃ m,
+        find_fresh_string c n = cand m ∧
+        (n ≤ m)%N ∧
+        cand m ∉ c ∧
+        ∀ i, (n ≤ i < m)%N → cand i ∈ c.
+  Proof.
+    unfold find_fresh_string.
+    induction c as [c IH] using (well_founded_ind collection_wf).
+    intro.
+    rewrite (set_recursion_unfold' (pointwise_relation N eq)).
+    2: intros * eqg i; destruct decide; auto; apply eqg.
+    destruct decide as [case|case].
+    - destruct (IH _ (subset_difference_in case) (1+n)%N) as [m [eqrec [bound [notin inlow]]]].
+      exists m; repeat (split; auto).
+      + lia.
+      + contradict notin.
+        rewrite elem_of_difference; split; auto.
+        rewrite elem_of_singleton /cand.
+        intros ?%string_app_inj%pretty_N_inj; lia.
+      + intros i [lb ub].
+        destruct (decide (i = n)) as [<-|neq]; auto.
+        enough (cand i ∈ c ∖ {[ cand n ]}) as [??]%elem_of_difference by done.
+        apply inlow; lia.
+    - exists n; repeat split; auto.
+      intros; lia.
+  Qed.
+End FreshString.
+
+Instance fresh_string `{FinCollection string C} `{InDec: ∀ (x: string) (s: C), Decision (x ∈ s)}:
+  Fresh string C := λ c, find_fresh_string "~" c 0%N.
+Instance fresh_string_spec `{FinCollection string C} `{InDec: ∀ (x: string) (s: C), Decision (x ∈ s)}:
+  FreshSpec string C.
+Proof.
+  split.
+  - apply _.
+  - intros * eqXY.
+    pose proof (find_fresh_string_spec "~" X 0%N) as specX.
+    pose proof (find_fresh_string_spec "~" Y 0%N) as specY.
+    unfold fresh, fresh_string.
+    destruct specX as [mX [-> [_ [notinX inX]]]].
+    destruct specY as [mY [-> [_ [notinY inY]]]].
+    destruct (N.lt_trichotomy mX mY) as [case|[->|case]].
+    2: done.
+    + contradict notinX.
+      rewrite eqXY.
+      apply inY; lia.
+    + contradict notinY.
+      rewrite -eqXY.
+      apply inX; lia.
+  - intros.
+    unfold fresh, fresh_string.
+    destruct (find_fresh_string_spec "~" X 0%N) as [m [-> [_ [? _]]]]; auto.
+Qed.
